src/GC.fst
@@ -789,3 +789,4 @@ let assign_pres_equiv cs bs l bexp init =
         assert(equiv_state cs'' bs' init);
         garbageCollect_pres_equiv cs'' bs' bit init
 
+
